Very small edits. In the end, it turns out that provable_iffp can be unrewritable if types are complicated, although it is rewrittable with simpler types. See LogicGenerator/demo/test.v.

LogicGenerator/demo/implementation_6.v
@@ -2,6 +2,8 @@ Require Import HypotheticalExternLib.
 Require Import ZArith.
 Require Import interface_6.
 
+Definition RealProvable `{para} (e: (nat -> option X) -> Prop) := forall st, e st.
+
 Module NaiveLang.
   Definition expr `{para} := (nat -> option X) -> Prop.
   Section NaiveLang.
@@ -25,7 +27,7 @@ Module NaiveLang.
     forall p, st p = None.
   Definition corable (e: expr): Prop := forall s1 s2, e s1 <-> e s2.
   
-  Definition provable (e : expr) : Prop := forall st, e st.
+  Definition provable := RealProvable.
   End NaiveLang.
 End NaiveLang.
 
@@ -36,49 +38,49 @@ Module NaiveRule.
 
   Lemma modus_ponens :
     forall x y : expr, provable (impp x y) -> provable x -> provable y.
-  Proof. unfold provable, impp. auto. Qed.
+  Proof. unfold provable, RealProvable, impp. auto. Qed.
 
   Lemma axiom1 : forall x y : expr, provable (impp x (impp y x)).
-  Proof. unfold provable, impp. auto. Qed.
+  Proof. unfold provable, RealProvable, impp. auto. Qed.
 
   Lemma axiom2 : forall x y z : expr,
       provable (impp (impp x (impp y z)) (impp (impp x y) (impp x z))).
-  Proof. unfold provable, impp. auto. Qed.
+  Proof. unfold provable, RealProvable, impp. auto. Qed.
 
   Lemma andp_intros :
     forall x y : expr, provable (impp x (impp y (andp x y))).
-  Proof. unfold provable, impp, andp. auto. Qed.
+  Proof. unfold provable, RealProvable, impp, andp. auto. Qed.
 
   Lemma andp_elim1 : forall x y : expr, provable (impp (andp x y) x).
-  Proof. unfold provable, impp, andp. tauto. Qed.
+  Proof. unfold provable, RealProvable, impp, andp. tauto. Qed.
 
   Lemma andp_elim2 : forall x y : expr, provable (impp (andp x y) y).
-  Proof. unfold provable, impp, andp. tauto. Qed.
+  Proof. unfold provable, RealProvable, impp, andp. tauto. Qed.
 
   Lemma orp_intros1 : forall x y : expr, provable (impp x (orp x y)).
-  Proof. unfold provable, impp, orp. auto. Qed.
+  Proof. unfold provable, RealProvable, impp, orp. auto. Qed.
 
   Lemma orp_intros2 : forall x y : expr, provable (impp y (orp x y)).
-  Proof. unfold provable, impp, orp. auto. Qed.
+  Proof. unfold provable, RealProvable, impp, orp. auto. Qed.
 
   Lemma orp_elim : forall x y z : expr,
       provable (impp (impp x z) (impp (impp y z) (impp (orp x y) z))).
-  Proof. unfold provable, impp, orp. tauto. Qed.
+  Proof. unfold provable, RealProvable, impp, orp. tauto. Qed.
 
   Lemma falsep_elim : forall x : expr, provable (impp falsep x).
-  Proof. unfold provable, impp, falsep. destruct 1. Qed.
+  Proof. unfold provable, RealProvable, impp, falsep. destruct 1. Qed.
 
   Lemma excluded_middle : forall x : expr, provable (orp x (negp x)).
-  Proof. unfold provable, orp, negp, impp, falsep. intros; tauto. Qed.
+  Proof. unfold provable, RealProvable, orp, negp, impp, falsep. intros; tauto. Qed.
 
   Lemma coq_prop_intros : (forall P : Prop, P -> provable (coq_prop P)) .
-  Proof. unfold provable, coq_prop. intros; tauto. Qed.
+  Proof. unfold provable, RealProvable, coq_prop. intros; tauto. Qed.
   
   Lemma coq_prop_elim : (forall (P : Prop) (x : expr), (P -> provable x) -> provable (impp (coq_prop P) x)) .
-  Proof. unfold provable, impp, coq_prop. intros; auto. Qed.
+  Proof. unfold provable, RealProvable, impp, coq_prop. intros; auto. Qed.
     
   Lemma coq_prop_impp : (forall P Q : Prop, provable (impp (impp (coq_prop P) (coq_prop Q)) (coq_prop (P -> Q)))) .
-  Proof. unfold provable, impp, coq_prop. intros; auto. Qed.
+  Proof. unfold provable, RealProvable, impp, coq_prop. intros; auto. Qed.
   
   Axiom sepcon_comm: forall x y, provable (iffp (sepcon x y) (sepcon y x)).
   Axiom sepcon_assoc: forall x y z,
